Dumping a bunch of work.  Pretty broken at the moment.

SeqNatToNat.dfy
@@ -1,4 +1,525 @@
+include "../libraries/src/Wrappers.dfy"
+
 module SeqNatToNat {
 
-  
+  import opened Wrappers
+
+  // Define functions that take a Seq<nat> and convert it
+  // reversibly to a single nat.
+
+  // The approach take is to:
+  // 1) Split each nat into bits (Seq<bool).
+  // 2) Interleave those bits.
+  // 3) Convert the bits back into a new nat.
+
+  // Pop a bit off a nat (lsb).
+  function PopBit(n: nat): (r: (bool, nat))
+  {
+    var b := n % 2 == 1;
+    (b, if b then (n-1)/2 else n/2)
+  }
+
+  // Push a bit onto a nat (lsb).
+  function PushBit(b: bool, n: nat): (r: nat)
+  {
+    (if b then 1 else 0) + 2 * n
+  }
+
+  function divmod(n: nat, d: nat): (r: (nat, nat))
+    requires d > 0
+    decreases n
+    ensures n == r.0 + r.1*d
+    ensures r.0 < d
+  {
+    if n < d then
+      (n, 0)
+    else
+      var (r1, r2) := divmod(n-d, d);
+      (r1, r2+1)
+  }
+
+  function divmodinv(rem: nat, quot: nat, d: nat): nat
+    requires rem < d
+    requires d > 0
+  {
+    rem + quot * d
+  }
+
+  lemma RemoveLTFactor(a: nat, b: nat, f: nat)
+    requires a*f < b*f
+    ensures a < b
+  {
+  }
+
+  lemma divmodUnique(rem1: nat, quot1: nat, rem2: nat, quot2: nat, d: nat)
+    requires d > 0
+    requires rem1 < d
+    requires rem2 < d
+    requires divmodinv(rem1, quot1, d) == divmodinv(rem2, quot2, d)
+    ensures rem1 == rem2
+    ensures quot1 == quot2
+  {
+    var n := divmodinv(rem1, quot1, d);
+    assert n == divmodinv(rem2, quot2, d);
+    assert n < d+quot2*d;
+    assert n < d+quot1*d;
+    assert n >= quot2*d;
+    assert n >= quot1*d;
+    assert quot1*d < d+quot2*d;
+    RemoveLTFactor(quot1, 1+quot2, d);
+    assert quot1 < 1+quot2;
+    assert quot2*d < d+quot1*d;
+    RemoveLTFactor(quot2, 1+quot1, d);
+    assert quot2 < 1+quot1;
+    assert quot1 == quot2;
+    assert rem1+quot1*d == rem2+quot2*d;
+    assert rem1 == rem2;
+  }
+
+  lemma divmodinvdivmod(rem: nat, quot: nat, d: nat)
+    requires rem < d
+    requires d > 0
+    ensures
+      var n := divmodinv(rem, quot, d);
+      divmod(n, d) == (rem, quot)
+    decreases quot
+  {
+      var n := divmodinv(rem, quot, d);
+      assert n == rem + quot*d;
+      if n < d {
+        assert divmod(n, d) == (rem, quot);
+      } else {
+        var (rem2, quot2) := divmod(n-d, d);
+        divmodinvdivmod(rem2, quot2, d);
+        assert divmod(n-d, d) == (rem2, quot2);
+        assert divmod(n, d) == (rem2, quot2+1);
+        assert n-d == rem2 + quot2*d;
+        assert n == rem2 + (quot2+1)*d;
+        divmodUnique(rem, quot, rem2, quot2+1, d);
+        assert rem == rem2;
+        assert quot == quot2+1;
+        assert divmod(n, d) == (rem, quot);
+      }
+
+  }
+
+  lemma divmodDecreases(n: nat, d: nat)
+    requires d > 1
+    requires n > 0
+    ensures
+      var (r, q) := divmod(n, d);
+      q < n
+    decreases n
+  {
+  }
+
+  lemma PushPop(b: bool, n: nat)
+    ensures
+      var r := PushBit(b, n);
+      PopBit(r) == (b, n)
+  {
+  }
+
+  function BitsToNat(ns: seq<bool>): (r: nat)
+    decreases |ns|
+    ensures r < pow2(|ns|)
+  {
+    if |ns| == 0 then
+      0
+    else
+      var h := ns[0];
+      var t: nat := BitsToNat(ns[1..]);
+      PushBit(h, t)
+  }
+
+  function BitsToNatRev(ns: seq<bool>): (r: nat)
+    decreases |ns|
+    ensures r < pow2(|ns|)
+  {
+    if |ns| == 0 then
+      0
+    else
+      var h := ns[|ns|-1];
+      var t := BitsToNatRev(ns[..|ns|-1]);
+      t + if h then pow2(|ns|-1) else 0
+  }
+
+  //lemma BitsToNatEquiv(ns: seq<bool>)
+  //  ensures BitsToNat(ns) == BitsToNatRev(ns)
+  //{
+  //}
+
+  lemma BitsToNatNotZero(ns: seq<bool>)
+    requires exists index: nat :: index < |ns| && ns[index]
+    ensures BitsToNat(ns) > 0
+  {
+  }
+
+  function NatToBits(n: nat, l: nat): (r: seq<bool>)
+    requires n < pow2(l)
+    ensures |r| == l
+  {
+    if l == 0 then
+      []
+    else
+      var (h, t) := PopBit(n);
+      [h] + NatToBits(t, l-1)
+  }
+
+  lemma BitsToNatToBits(ns: seq<bool>)
+    ensures NatToBits(BitsToNat(ns), |ns|) == ns
+    decreases |ns|
+  {
+    if |ns| == 0 {
+      var n: nat := BitsToNat(ns);
+      var r: seq<bool> := NatToBits(n, |ns|);
+      assert r == ns;
+    } else {
+      var new_ns := NatToBits(BitsToNat(ns), |ns|);
+      assert new_ns == NatToBits(PushBit(ns[0], BitsToNat(ns[1..])), |ns|);
+      var (h, t) := PopBit(PushBit(ns[0], BitsToNat(ns[1..])));
+      PushPop(ns[0], BitsToNat(ns[1..]));
+      assert h == ns[0];
+      assert t == BitsToNat(ns[1..]);
+      assert new_ns == [h] + NatToBits(BitsToNat(ns[1..]), |ns|-1);
+      BitsToNatToBits(ns[1..]);
+      assert new_ns == [h] + ns[1..];
+      assert new_ns == ns;
+    }
+  }
+
+  lemma {:vcs_split_on_every_assert} NatToBitsToNat(n: nat, l: nat)
+    requires n < pow2(l)
+    ensures BitsToNat(NatToBits(n, l)) == n
+    decreases l
+  {
+    if l == 0 {
+      assert n == 0;
+      assert BitsToNat(NatToBits(n, l)) == n;
+    } else {
+      var b := n % 2 == 1;
+      var new_n := if b then (n-1)/2 else n/2;
+      calc {
+        BitsToNat(NatToBits(n, l));
+        BitsToNat([b] + NatToBits(new_n, l-1));
+        n % 2 + 2*BitsToNat(NatToBits(new_n, l-1));
+        {NatToBitsToNat(new_n, l-1);}
+        n % 2 + 2*new_n;
+        n;
+      }
+    }
+  }
+
+  function ShiftLeftOne(n: nat): (r: nat)
+  {
+    if n % 2 == 0 then
+      n/2
+    else
+      (n-1)/2
+  }
+
+  lemma SplitLowestBit(n: nat)
+    ensures n == n % 2 + 2*ShiftLeftOne(n)
+  {
+  }
+
+  lemma IsLowestBit(n: nat, a: nat, b: nat)
+    requires a < 2
+    requires n == a + 2 * b
+    ensures a == n % 2
+  {
+  }
+
+  function Max(ns: seq<nat>): (r: nat)
+    requires |ns| > 0
+    ensures r in ns
+    ensures forall index: nat | index < |ns| :: ns[index] <= r
+  {
+    if |ns| == 1 then
+      ns[0]
+    else
+      var max_later := Max(ns[1..]);
+      if ns[0] > max_later then
+        ns[0]
+      else
+        max_later
+  }
+
+  function pow2(n: nat): (r: nat)
+    ensures r > 0
+    decreases n
+  {
+    if n == 0 then
+      1
+    else
+      2 * pow2(n-1)
+  }
+
+  function {:opaque} PopLowBits(ns: seq<nat>): (r: seq<bool>)
+    requires |ns| > 0
+    ensures |r| == |ns|
+  {
+    seq(|ns|, i requires 0<= i < |ns| => ns[i] % 2 == 1)
+  }
+
+  predicate HasTrueElement(b: seq<bool>)
+  {
+    exists index: nat :: index < |b| && b[index]
+  }
+
+  lemma PopLowBitsMaxOne(ns: seq<nat>)
+    requires |ns| > 0
+    requires Max(ns) == 1
+    ensures
+      var r := PopLowBits(ns);
+      HasTrueElement(r)
+  {
+    var r := PopLowBits(ns);
+    var index: nat :| index < |ns| && ns[index] == Max(ns);
+    reveal PopLowBits();
+    assert r[index];
+    assert HasTrueElement(r);
+  }
+
+  function {:opaque} PopUpperBits(ns: seq<nat>): (r: seq<nat>)
+    requires |ns| > 0
+    ensures |r| == |ns|
+    ensures Max(ns) > 0 ==> Max(r) < Max(ns)
+  {
+    seq(|ns|, i requires 0 <= i < |ns| => ShiftLeftOne(ns[i]))
+  }
+
+  lemma PopUpperBitsNonZero(ns: seq<nat>)
+    requires |ns| > 0
+    requires Max(ns) > 1
+    ensures Max(PopUpperBits(ns)) > 0
+  {
+    var r := PopUpperBits(ns);
+    var max_index: nat :| max_index < |ns| && ns[max_index] == Max(ns);
+    reveal PopUpperBits();
+    assert r[max_index] == ShiftLeftOne(ns[max_index]);
+  }
+
+  function NatsToNat(ns: seq<nat>): (r: nat)
+    requires |ns| > 0
+    decreases Max(ns)
+  {
+    var max := Max(ns);
+    if max == 0 then
+      0
+    else
+      var line := PopLowBits(ns);
+      var reduced_ns := PopUpperBits(ns);
+      divmodinv(BitsToNat(line), NatsToNat(reduced_ns), pow2(|ns|))
+  }
+
+  function {:opaque} PushBits(head: seq<bool>, tail: seq<nat>): (r: seq<nat>)
+    requires |head| == |tail|
+    ensures |r| == |head|
+  {
+      var l := |head|;
+      seq(l, i requires 0 <= i < l => (if head[i] then 1 else 0) + 2*tail[i])
+  }
+
+  function NatToNats(n: nat, l: nat): (r: seq<nat>)
+    requires l > 0
+    decreases n
+  {
+    if n == 0 then
+      seq(l, i requires 0 <= i < l => 0)
+    else
+      assert pow2(l) > 1;
+      var (rem, quot) := divmod(n, pow2(l));
+      var head: seq<bool> := NatToBits(rem, l);
+      assert |head| == l;
+      var tail: seq<nat> := NatToNats(quot, l);
+      assert |tail| == l;
+      PushBits(head, tail)
+  }
+
+  lemma NatsToNatToNatsPartial(ns: seq<nat>)
+    requires |ns| > 0
+    ensures PushBits(PopLowBits(ns), PopUpperBits(ns)) == ns
+  {
+      var line := PopLowBits(ns);
+      var reduced_ns := PopUpperBits(ns);
+      reveal PopLowBits();
+      reveal PopUpperBits();
+      reveal PushBits();
+      var merged := PushBits(line, reduced_ns);
+      assert merged == ns;
+  }
+
+  lemma MultBothGreaterZero(a: nat, b: nat)
+    requires a > 0
+    requires b > 0
+    ensures a * b > 0
+  {
+  }
+
+  predicate AllZeros(ns: seq<nat>)
+  {
+    forall i: nat :: i < |ns| ==> ns[i] == 0
+  }
+
+  lemma TrueGivesNonZero(n: nat, l: nat)
+    requires n < pow2(l)
+    requires true in NatToBits(n, l)
+    ensures n > 0
+  {
+  }
+
+  lemma AllFalseGivesZero(n: nat, l: nat)
+    requires n < pow2(l)
+    requires !(true in NatToBits(n, l))
+    ensures n == 0
+  {
+  }
+
+  lemma {:vcs_split_on_every_assert} NatToNatsNonZero(n: nat, l: nat)
+    requires n > 0
+    requires l > 0
+    ensures Max(NatToNats(n, l)) > 0
+  {
+    assert pow2(l) > 1;
+    var exn := NatToNats(n, l);
+    var (rem, quot) := divmod(n, pow2(l));
+    assert rem < pow2(l);
+    var head: seq<bool> := NatToBits(rem, l);
+    assert |head| == l;
+    var tail: seq<nat> := NatToNats(quot, l);
+    assert |tail| == l;
+    var expanded := PushBits(head, tail);
+    assert expanded == NatToNats(n, l);
+    reveal PushBits();
+    if true in head {
+      TrueGivesNonZero(rem, l);
+      assert rem > 0;
+      var index: nat :| index < l && head[index];
+      assert expanded[index] > 0;
+      assert Max(NatToNats(n, l)) > 0;
+    } else {
+      AllFalseGivesZero(rem, l);
+      assert rem == 0;
+      assert quot > 0;
+      NatToNatsNonZero(quot, l);
+      assert Max(tail) > 0;
+      var index: nat :| index < l && tail[index] > 0;
+      assert expanded[index] > 0;
+      assert Max(NatToNats(n, l)) > 0;
+    }
+  }
+
+  lemma {:vcs_split_on_every_assert} NatsToNatNonZero(ns: seq<nat>)
+    requires |ns| > 0
+    requires Max(ns) > 0
+    ensures NatsToNat(ns) > 0
+    decreases Max(ns)
+  {
+      var max := Max(ns);
+      var max_index: nat :| max_index < |ns| && ns[max_index] == max;
+      var line := PopLowBits(ns);
+      var reduced_ns := PopUpperBits(ns);
+      if max == 1 {
+        PopLowBitsMaxOne(ns);
+        BitsToNatNotZero(line);
+        assert BitsToNat(line) > 0;
+      } else {
+        PopUpperBitsNonZero(ns);
+        NatsToNatNonZero(reduced_ns);
+        assert NatsToNat(reduced_ns) > 0;
+      }
+      assert NatsToNat(ns) == divmodinv(BitsToNat(line), NatsToNat(reduced_ns), pow2(|ns|));
+      if max == 1 {
+        assert BitsToNat(line) > 0;
+        assert NatsToNat(ns) > 0;
+      } else {
+        assert NatsToNat(reduced_ns) > 0;
+        assert pow2(|ns|) > 0;
+        MultBothGreaterZero(pow2(|ns|), NatsToNat(reduced_ns));
+        assert pow2(|ns|)*NatsToNat(reduced_ns) > 0;
+        assert NatsToNat(ns) > 0;
+      }
+
+  }
+
+  lemma {:vcs_split_on_every_assert} NatsToNatToNats(ns: seq<nat>)
+    requires |ns| > 0
+    ensures NatToNats(NatsToNat(ns), |ns|) == ns
+    decreases Max(ns)
+  {
+    if Max(ns) == 0 {
+      assert NatsToNat(ns) == 0;
+      assert NatToNats(NatsToNat(ns), |ns|) == ns;
+    } else {
+      var n := NatsToNat(ns);
+      NatsToNatNonZero(ns);
+      assert n > 0;
+      var l := |ns|;
+      var line := PopLowBits(ns);
+      var reduced_ns := PopUpperBits(ns);
+      assert n == divmodinv(BitsToNat(line), NatsToNat(reduced_ns), pow2(l));
+      var (rem, quot) := divmod(n, pow2(l));
+      divmodUnique(rem, quot, BitsToNat(line), NatsToNat(reduced_ns), pow2(l));
+      var new_ns := NatToNats(NatsToNat(ns), |ns|);
+      assert new_ns == NatToNats(divmodinv(BitsToNat(line), NatsToNat(reduced_ns), pow2(l)), l);
+      assert new_ns == NatToNats(divmodinv(rem, quot, pow2(l)), l);
+      var head: seq<bool> := NatToBits(rem, l);
+      assert |head| == l;
+      var tail: seq<nat> := NatToNats(quot, l);
+      assert new_ns == PushBits(head, tail);
+      assert head == NatToBits(BitsToNat(line), l);
+      BitsToNatToBits(line);
+      assert head == line;
+      NatsToNatToNats(reduced_ns);
+      assert tail == NatToNats(NatsToNat(reduced_ns), l);
+      assert tail == reduced_ns;
+      assert new_ns == PushBits(line, reduced_ns);
+      assert new_ns == PushBits(PopLowBits(ns), PopUpperBits(ns));
+      NatsToNatToNatsPartial(ns);
+      assert new_ns == ns;
+    }
+  }
+
+  lemma NatToNatsToNatPartial(head: seq<bool>, tail: seq<nat>)
+    requires |head| > 0
+    requires |head| == |tail|
+    ensures PopLowBits(PushBits(head, tail)) == head
+    ensures PopUpperBits(PushBits(head, tail)) == tail
+  {
+      reveal PushBits();
+      reveal PopLowBits();
+      reveal PopUpperBits();
+  }
+
+  lemma {:vcs_split_on_every_assert} NatToNatsToNat(n: nat, l: nat)
+    requires l > 0
+    ensures NatsToNat(NatToNats(n, l)) == n
+    decreases n
+  {
+    if n == 0 {
+        assert NatsToNat(NatToNats(n, l)) == n;
+    } else {
+        var ns := NatToNats(n, l);
+        NatToNatsNonZero(n, l);
+        assert Max(ns) > 0;
+        var new_n := NatsToNat(NatToNats(n, l));
+        var (rem, quot) := divmod(n, pow2(l));
+        var head: seq<bool> := NatToBits(rem, l);
+        var tail: seq<nat> := NatToNats(quot, l);
+        assert new_n == NatsToNat(PushBits(head, NatToNats(quot, l)));
+        assert ns == PushBits(head, NatToNats(quot, l));
+        NatToNatsToNatPartial(head, tail);
+        assert PopLowBits(ns) == head;
+        assert PopUpperBits(ns) == tail;
+        assert new_n == divmodinv(BitsToNat(head), NatsToNat(tail), pow2(l));
+        NatToNatsToNat(quot, l);
+        assert NatsToNat(NatToNats(quot, l)) == quot;
+        assert new_n == divmodinv(BitsToNat(head), quot, pow2(l));
+        NatToBitsToNat(rem, l);
+        assert new_n == divmodinv(rem, quot, pow2(l));
+        assert NatsToNat(NatToNats(n, l)) == n;
+    }
+  }
+    
 }
